Clean/Circuit/Explicit.lean
@@ -412,6 +412,9 @@ instance {M : TypeMap} [ProvableType M] (c : Var (UnconstrainedDep M) F) :
   channelsWithGuarantees _ := []
   channelsWithRequirements _ := []
 
+instance {F : Type} [Field F] (x : Var (UnconstrainedDep field) F) : ExplicitCircuit (witnessVar x) :=
+  ExplicitCircuits.toSingle _ _ (explicit := inferInstanceAs (ExplicitCircuits witnessVar))
+
 instance {value var : TypeMap} [ProvableType value] [inst : Witnessable F value var] :
     ExplicitCircuits (witness (F:=F) (value:=value) (var:=var)) where
   output _ n := inst.var_eq ▸ varFromOffset value n
